added more verified functions (#400)

Test/inst/vector.bpl
@@ -36,16 +36,20 @@ function {:inline} Vec_Remove<T>(v: Vec T): Vec T {
     else Vec_Empty()
 }
 
-procedure Vec_Ext(A: Vec int, B: Vec int) returns (i: int);
+type Element;
+
+// extensionality lemma to be used explicitly by the programmer
+procedure Vec_Ext(A: Vec Element, B: Vec Element) returns (i: int);
 ensures A == B || Vec_Len(A) != Vec_Len(B) || Vec_Nth(A, i) != Vec_Nth(B, i);
 
-procedure Ex0(A: Vec int, i: int)
+// procedures Ex0 to Ex9 are exercises to ramp up to the "real" vector procedures
+procedure Ex0(A: Vec Element, i: int)
 requires 0 <= i && i < Vec_Len(A);
 {
     assert Vec_Concat(Vec_Slice(A, 0, i), Vec_Slice(A, i, Vec_Len(A))) == A;
 }
 
-procedure Ex1(A: Vec int, i: int)
+procedure Ex1(A: Vec Element, i: int)
 requires 0 <= i && i < Vec_Len(A) - 1;
 requires Vec_Nth(A, i) == Vec_Nth(A, i + 1);
 {
@@ -57,7 +61,7 @@ requires Vec_Nth(A, i) == Vec_Nth(A, i + 1);
     assert Vec_Swap(A, i, i+1) == A;
 }
 
-procedure Ex2(A: Vec int, i: int, j: int)
+procedure Ex2(A: Vec Element, i: int, j: int)
 requires 0 <= i && i < Vec_Len(A);
 requires 0 <= j && j < Vec_Len(A);
 requires Vec_Nth(A, i) == Vec_Nth(A, j);
@@ -65,7 +69,7 @@ requires Vec_Nth(A, i) == Vec_Nth(A, j);
     assert Vec_Swap(A, i, j) == A;
 }
 
-procedure Ex3(A: Vec int, i: int, j: int)
+procedure Ex3(A: Vec Element, i: int, j: int)
 requires 0 <= i && i < Vec_Len(A);
 requires 0 <= j && j < Vec_Len(A);
 {
@@ -75,11 +79,11 @@ requires 0 <= j && j < Vec_Len(A);
     Vec_Concat(Vec_Slice(A, 0, j), Vec_Slice(A, j, Vec_Len(A)));
 }
 
-procedure Ex4(A: Vec int, B: Vec int, i: int, e: int)
+procedure Ex4(A: Vec Element, B: Vec Element, i: int, e: Element)
 requires 0 <= i && i < Vec_Len(A);
 requires Vec_Concat(Vec_Slice(A, 0, i), Vec_Slice(A, i + 1, Vec_Len(A))) == B;
 {
-    var A', B': Vec int;
+    var A', B': Vec Element;
 
     A' := Vec_Append(A, e);
     B' := Vec_Append(B, e);
@@ -87,12 +91,12 @@ requires Vec_Concat(Vec_Slice(A, 0, i), Vec_Slice(A, i + 1, Vec_Len(A))) == B;
     assert Vec_Concat(Vec_Slice(A', 0, i), Vec_Slice(A', i + 1, Vec_Len(A'))) == B';
 }
 
-procedure Ex5(A: Vec int, B: Vec int, i: int, e: int)
+procedure Ex5(A: Vec Element, B: Vec Element, i: int, e: Element)
 requires 0 <= i && i < Vec_Len(A);
 requires Vec_Nth(A, i) == Vec_Nth(B, Vec_Len(B) - 1);
 requires Vec_Concat(Vec_Slice(A, 0, i), Vec_Slice(A, i + 1, Vec_Len(A))) == Vec_Slice(B, 0, Vec_Len(B) - 1);
 {
-    var A', B': Vec int;
+    var A', B': Vec Element;
 
     A' := Vec_Append(A, e);
     B' := Vec_Swap(Vec_Append(B, e), Vec_Len(B) - 1, Vec_Len(B));
@@ -101,12 +105,12 @@ requires Vec_Concat(Vec_Slice(A, 0, i), Vec_Slice(A, i + 1, Vec_Len(A))) == Vec_
     Vec_Nth(Vec_Concat(Vec_Slice(A', 0, i), Vec_Slice(A', i + 1, Vec_Len(A'))), x) == Vec_Nth(Vec_Slice(B', 0, Vec_Len(B') - 1), x));
 }
 
-procedure Ex6a(A: Vec int, B: Vec int, i: int, e: int)
+procedure Ex6a(A: Vec Element, B: Vec Element, i: int, e: Element)
 requires 0 <= i && i < Vec_Len(A);
 requires Vec_Nth(A, i) == Vec_Nth(B, Vec_Len(B) - 1);
 requires Vec_Concat(Vec_Slice(A, 0, i), Vec_Slice(A, i + 1, Vec_Len(A))) == Vec_Slice(B, 0, Vec_Len(B) - 1);
 {
-    var A', B': Vec int;
+    var A', B': Vec Element;
 
     A' := Vec_Append(A, e);
     B' := Vec_Swap(Vec_Append(B, e), Vec_Len(B) - 1, Vec_Len(B));
@@ -114,12 +118,12 @@ requires Vec_Concat(Vec_Slice(A, 0, i), Vec_Slice(A, i + 1, Vec_Len(A))) == Vec_
     assert Vec_Nth(A', i) == Vec_Nth(B', Vec_Len(B') - 1);
 }
 
-procedure Ex6b(A: Vec int, B: Vec int, i: int, e: int)
+procedure Ex6b(A: Vec Element, B: Vec Element, i: int, e: Element)
 requires 0 <= i && i < Vec_Len(A);
 requires Vec_Nth(A, i) == Vec_Nth(B, Vec_Len(B) - 1);
 requires Vec_Concat(Vec_Slice(A, 0, i), Vec_Slice(A, i + 1, Vec_Len(A))) == Vec_Slice(B, 0, Vec_Len(B) - 1);
 {
-    var A', B': Vec int;
+    var A', B': Vec Element;
     var x: int;
 
     A' := Vec_Append(A, e);
@@ -130,13 +134,13 @@ requires Vec_Concat(Vec_Slice(A, 0, i), Vec_Slice(A, i + 1, Vec_Len(A))) == Vec_
     Vec_Concat(Vec_Slice(A', 0, i), Vec_Slice(A', i + 1, Vec_Len(A'))) == Vec_Slice(B', 0, Vec_Len(B') - 1);
 }
 
-procedure Ex7a(A: Vec int, j: int, B: Vec int, i: int)
+procedure Ex7a(A: Vec Element, j: int, B: Vec Element, i: int)
 requires 0 <= j && j <= i && i < Vec_Len(A) - 1;
 requires Vec_Nth(B, i) == Vec_Nth(A, j);
 requires Vec_Slice(B, 0, i) == Vec_Concat(Vec_Slice(A, 0, j), Vec_Slice(A, j + 1, i + 1));
 requires Vec_Slice(B, i + 1, Vec_Len(B)) == Vec_Slice(A, i + 1, Vec_Len(A));
 {
-    var B': Vec int;
+    var B': Vec Element;
     var i': int;
 
     B' := Vec_Swap(B, i, i + 1);
@@ -145,13 +149,13 @@ requires Vec_Slice(B, i + 1, Vec_Len(B)) == Vec_Slice(A, i + 1, Vec_Len(A));
     assert Vec_Nth(B', i') == Vec_Nth(A, j);
 }
 
-procedure Ex7b(A: Vec int, j: int, B: Vec int, i: int)
+procedure Ex7b(A: Vec Element, j: int, B: Vec Element, i: int)
 requires 0 <= j && j <= i && i < Vec_Len(A) - 1;
 requires Vec_Nth(B, i) == Vec_Nth(A, j);
 requires Vec_Slice(B, 0, i) == Vec_Concat(Vec_Slice(A, 0, j), Vec_Slice(A, j + 1, i + 1));
 requires Vec_Slice(B, i + 1, Vec_Len(B)) == Vec_Slice(A, i + 1, Vec_Len(A));
 {
-    var B': Vec int;
+    var B': Vec Element;
     var i': int;
     var x: int;
 
@@ -163,13 +167,13 @@ requires Vec_Slice(B, i + 1, Vec_Len(B)) == Vec_Slice(A, i + 1, Vec_Len(A));
     Vec_Slice(B', 0, i') == Vec_Concat(Vec_Slice(A, 0, j), Vec_Slice(A, j + 1, i' + 1));
 }
 
-procedure Ex7c(A: Vec int, j: int, B: Vec int, i: int)
+procedure Ex7c(A: Vec Element, j: int, B: Vec Element, i: int)
 requires 0 <= j && j <= i && i < Vec_Len(A) - 1;
 requires Vec_Nth(B, i) == Vec_Nth(A, j);
 requires Vec_Slice(B, 0, i) == Vec_Concat(Vec_Slice(A, 0, j), Vec_Slice(A, j + 1, i + 1));
 requires Vec_Slice(B, i + 1, Vec_Len(B)) == Vec_Slice(A, i + 1, Vec_Len(A));
 {
-    var B': Vec int;
+    var B': Vec Element;
     var i': int;
     var x: int;
 
@@ -181,8 +185,8 @@ requires Vec_Slice(B, i + 1, Vec_Len(B)) == Vec_Slice(A, i + 1, Vec_Len(A));
     Vec_Slice(B', i' + 1, Vec_Len(B')) == Vec_Slice(A, i' + 1, Vec_Len(A));
 }
 
-procedure Ex8(A: Vec int, j: int, B: Vec int, i: int)
-returns (B': Vec int, i': int)
+procedure Ex8(A: Vec Element, j: int, B: Vec Element, i: int)
+returns (B': Vec Element, i': int)
 requires 0 <= j && j <= i && i < Vec_Len(A) - 1;
 requires Vec_Nth(B, i) == Vec_Nth(A, j);
 requires Vec_Slice(B, 0, i) == Vec_Concat(Vec_Slice(A, 0, j), Vec_Slice(A, j + 1, i + 1));
@@ -206,7 +210,7 @@ ensures Vec_Slice(B', i' + 1, Vec_Len(B')) == Vec_Slice(A, i' + 1, Vec_Len(A));
     Vec_Slice(B', i' + 1, Vec_Len(B')) == Vec_Slice(A, i' + 1, Vec_Len(A));
 }
 
-procedure Ex9(A: Vec int, j: int) returns (B: Vec int, e: int)
+procedure Ex9(A: Vec Element, j: int) returns (B: Vec Element, e: Element)
 requires 0 <= j && j < Vec_Len(A);
 ensures e == Vec_Nth(A, j);
 ensures B == Vec_Concat(Vec_Slice(A, 0, j), Vec_Slice(A, j + 1, Vec_Len(A)));
@@ -232,7 +236,8 @@ ensures B == Vec_Concat(Vec_Slice(A, 0, j), Vec_Slice(A, j + 1, Vec_Len(A)));
     assert {:split_here} true;
 }
 
-procedure remove(A: Vec int, j: int) returns (B: Vec int, e: int)
+// "real" vector procedures start here
+procedure remove(A: Vec Element, j: int) returns (B: Vec Element, e: Element)
 requires 0 <= j && j < Vec_Len(A);
 ensures e == Vec_Nth(A, j);
 ensures B == Vec_Concat(Vec_Slice(A, 0, j), Vec_Slice(A, j + 1, Vec_Len(A)));
@@ -265,4 +270,112 @@ ensures B == Vec_Concat(Vec_Slice(A, 0, j), Vec_Slice(A, j + 1, Vec_Len(A)));
     call z := Vec_Ext(B, Vec_Concat(Vec_Slice(A, 0, j), Vec_Slice(A, j + 1, Vec_Len(A))));
     assume {:add_to_pool "Slice", z, j, j + 1, j - 1} true;
     assert {:split_here} true;
+}
+
+procedure swap_remove(A: Vec Element, j: int) returns (B: Vec Element)
+requires 0 <= j && j < Vec_Len(A);
+ensures Vec_Slice(B, 0, j) == Vec_Slice(A, 0, j);
+ensures Vec_Slice(B, j+1, Vec_Len(B)) == Vec_Slice(A, j+1, Vec_Len(B));
+ensures Vec_Nth(B, j) == Vec_Nth(A, Vec_Len(A) - 1);
+{
+    var last_idx: int;
+
+    last_idx := Vec_Len(A) - 1;
+    B := Vec_Swap(A, j, last_idx);
+    B := Vec_Remove(B);
+    assume {:add_to_pool "Slice", j, j + 1} true;
+}
+
+procedure reverse(A: Vec Element) returns (B: Vec Element)
+ensures Vec_Len(A) == Vec_Len(B);
+ensures (forall x: int :: 0 <= x && x < Vec_Len(A) ==> Vec_Nth(A, x) == Vec_Nth(B, Vec_Len(A) - 1 - x));
+{
+    var len: int;
+    var front_index: int;
+    var back_index: int;
+
+    B := A;
+    len := Vec_Len(A);
+    if (len == 0) {
+        return;
+    }
+
+    front_index := 0;
+    back_index := len - 1;
+    while (front_index < back_index)
+    invariant front_index + back_index == len - 1;
+    invariant Vec_Len(A) == Vec_Len(B);
+    invariant (forall x: int :: 0 <= x && x < front_index ==> Vec_Nth(A, x) == Vec_Nth(B, Vec_Len(A) - 1 - x));
+    invariant (forall x: int :: back_index < x && x < Vec_Len(A) ==> Vec_Nth(A, x) == Vec_Nth(B, Vec_Len(A) - 1 - x));
+    invariant (forall x: int :: front_index <= x && x <= back_index ==> Vec_Nth(A, x) == Vec_Nth(B, x));
+    {
+        B := Vec_Swap(B, front_index, back_index);
+        front_index := front_index + 1;
+        back_index := back_index - 1;
+    }
+}
+
+procedure append(A: Vec Element, B: Vec Element) returns (C: Vec Element)
+ensures C == Vec_Concat(A, B);
+{
+    var R: Vec Element;
+    var e: Element;
+    var y: int;
+
+    C := A;
+    call R := reverse(B);
+    while (0 < Vec_Len(R))
+    invariant (forall {:pool "L"} x: int :: {:skolem_add_to_pool "L", 0, x + 1}
+    0 <= x && x < Vec_Len(R) ==> Vec_Nth(B, x + Vec_Len(B) - Vec_Len(R)) == Vec_Nth(R, Vec_Len(R) - 1 - x));
+    invariant C == Vec_Concat(A, Vec_Slice(B, 0, Vec_Len(B) - Vec_Len(R)));
+    {
+        e := Vec_Nth(R, Vec_Len(R) - 1);
+        C := Vec_Append(C, e);
+        R := Vec_Remove(R);
+        assert Vec_Len(C) == Vec_Len(Vec_Concat(A, Vec_Slice(B, 0, Vec_Len(B) - Vec_Len(R))));
+        call y := Vec_Ext(C, Vec_Concat(A, Vec_Slice(B, 0, Vec_Len(B) - Vec_Len(R))));
+        assume {:add_to_pool "Slice", y, y - Vec_Len(A)} true;
+    }
+}
+
+procedure contains(A: Vec Element, e: Element) returns (found: bool)
+ensures !found <==> (forall x: int :: 0 <= x && x < Vec_Len(A) ==> Vec_Nth(A, x) != e);
+{
+    var i: int;
+    var len: int;
+
+    found := false;
+    i := 0;
+    len := Vec_Len(A);
+    while (i < len)
+    invariant 0 <= i;
+    invariant (forall x: int :: 0 <= x && x < i ==> Vec_Nth(A, x) != e);
+    {
+        if (Vec_Nth(A, i) == e) {
+            found := true;
+            return;
+        }
+        i := i + 1;
+    }
+}
+
+procedure index_of(A: Vec Element, e: Element) returns (found: bool, pos: int)
+ensures found ==> Vec_Nth(A, pos) == e;
+ensures !found ==> pos == 0 && (forall x: int :: 0 <= x && x < Vec_Len(A) ==> Vec_Nth(A, x) != e);
+{
+    var i: int;
+    var len: int;
+
+    found, pos := false, 0;
+    i := 0;
+    len := Vec_Len(A);
+    while (i < len)
+    invariant (forall x: int :: 0 <= x && x < i ==> Vec_Nth(A, x) != e);
+    {
+        if (Vec_Nth(A, i) == e) {
+            found, pos := true, i;
+            return;
+        }
+        i := i + 1;
+    }
 }
